impl init time out

concurrency/disciplined/CapacityAllocator.i.dfy
@@ -22,6 +22,7 @@ module CapacityAllocator {
   import opened NonlinearLemmas
   import opened CapacityAllocatorTypes
   import opened Count
+  import opened ShardedHashTable
 
   type AllocatorMutex = Mutex<AllocatorBin>
   type AllocatorMutexTable = seq<AllocatorMutex>
@@ -43,8 +44,6 @@ module CapacityAllocator {
     && |o| == NumberOfBins()
     && (forall i | 0 <= i < NumberOfBins() :: o[i].inv == BinInv)
   }
-
-  function Capacity() : nat
 
   function method CapacityImpl(): (s: uint32)
     ensures s as nat == Capacity()
